SyBloc/SBSemantics.v
@@ -2,31 +2,27 @@ Require Import List.
 Import List.ListNotations.
 Open Scope list_scope.
 
-(* Require Import Coq.Sorting.Permutation. *)
 Require Import Setoid.
 Require Import Morphisms.
-(* Require Import Coq.Arith.EqNat. *)
 
-(* Require Import Coq.FSets.FMapPositive. *)
 Require Import Velus.Common.
 Require Import Velus.Operators.
 Require Import Velus.Clocks.
 Require Import Velus.RMemory.
+Require Import Velus.NLustre.NLExprSyntax.
 Require Import Velus.SyBloc.SBSyntax.
-(* Require Import Velus.NLustre.Ordered. *)
+Require Import Velus.NLustre.NLExprSemantics.
 Require Import Velus.NLustre.Stream.
 
-
 Module Type SBSEMANTICS
-       (Import Ids   : IDS)
-       (Import Op    : OPERATORS)
-       (Import OpAux : OPERATORS_AUX Op)
-       (Import Clks  : CLOCKS    Ids)
-       (Import Syn   : SBSYNTAX  Ids Op Clks)
-       (Import Str   : STREAM        Op OpAux).
-
-  Definition env := PM.t value.
-  Definition history := PM.t (stream value).
+       (Import Ids     : IDS)
+       (Import Op      : OPERATORS)
+       (Import OpAux   : OPERATORS_AUX       Op)
+       (Import Clks    : CLOCKS          Ids)
+       (Import ExprSyn : NLEXPRSYNTAX        Op)
+       (Import Syn     : SBSYNTAX        Ids Op Clks ExprSyn)
+       (Import Str     : STREAM              Op OpAux)
+       (Import ExprSem : NLEXPRSEMANTICS Ids Op OpAux Clks ExprSyn Str).
 
   Record mvalue :=
     Mvalue { content_i: val;
@@ -41,298 +37,6 @@ Module Type SBSEMANTICS
   Definition memory := RMemory.memory mvalue.
   Definition memories := RMemory.memory mvalues.
 
-  (* Fixpoint find_init (x: ident) (mems: list (ident * const)): option const := *)
-  (*   match mems with *)
-  (*   | [] => None *)
-  (*   | m :: mems => *)
-  (*     if ident_eqb (fst m) x *)
-  (*     then Some (snd m) else find_init x mems *)
-  (*   end. *)
-
-  (** ** Instantaneous semantics *)
-
-  Section InstantSemantics.
-
-    Variable base: bool.
-    Variable R: env.
-
-    Inductive sem_var_instant: ident -> value -> Prop :=
-      Sv:
-        forall x v,
-          PM.find x R = Some v ->
-          sem_var_instant x v.
-
-    Definition sem_vars_instant (xs: list ident) (vs: list value) : Prop :=
-      Forall2 sem_var_instant xs vs.
-
-    Inductive sem_clock_instant: clock -> bool -> Prop :=
-    | Sbase:
-        sem_clock_instant Cbase base
-    | Son:
-        forall ck x c b,
-          sem_clock_instant ck true ->
-          sem_var_instant x (present c) ->
-          val_to_bool c = Some b ->
-          sem_clock_instant (Con ck x b) true
-    | Son_abs1:
-        forall ck x c,
-          sem_clock_instant ck false ->
-          sem_var_instant x absent ->
-          sem_clock_instant (Con ck x c) false
-    | Son_abs2:
-        forall ck x c b,
-          sem_clock_instant ck true ->
-          sem_var_instant x (present c) ->
-          val_to_bool c = Some b ->
-          sem_clock_instant (Con ck x (negb b)) false.
-
-    Inductive sem_lexp_instant: lexp -> value -> Prop:=
-    | Sconst:
-        forall c v,
-          v = (if base then present (sem_const c) else absent) ->
-          sem_lexp_instant (Econst c) v
-    | Svar:
-        forall x v ty,
-          sem_var_instant x v ->
-          sem_lexp_instant (Evar x ty) v
-    | Swhen_eq:
-        forall s x sc xc b,
-          sem_var_instant x (present xc) ->
-          sem_lexp_instant s (present sc) ->
-          val_to_bool xc = Some b ->
-          sem_lexp_instant (Ewhen s x b) (present sc)
-    | Swhen_abs1:
-        forall s x sc xc b,
-          sem_var_instant x (present xc) ->
-          val_to_bool xc = Some b ->
-          sem_lexp_instant s (present sc) ->
-          sem_lexp_instant (Ewhen s x (negb b)) absent
-    | Swhen_abs:
-        forall s x b,
-          sem_var_instant x absent ->
-          sem_lexp_instant s absent ->
-          sem_lexp_instant (Ewhen s x b) absent
-    | Sunop_eq:
-        forall le op c c' ty,
-          sem_lexp_instant le (present c) ->
-          sem_unop op c (typeof le) = Some c' ->
-          sem_lexp_instant (Eunop op le ty) (present c')
-    | Sunop_abs:
-        forall le op ty,
-          sem_lexp_instant le absent ->
-          sem_lexp_instant (Eunop op le ty) absent
-    | Sbinop_eq:
-        forall le1 le2 op c1 c2 c' ty,
-          sem_lexp_instant le1 (present c1) ->
-          sem_lexp_instant le2 (present c2) ->
-          sem_binop op c1 (typeof le1) c2 (typeof le2) = Some c' ->
-          sem_lexp_instant (Ebinop op le1 le2 ty) (present c')
-    | Sbinop_abs:
-        forall le1 le2 op ty,
-          sem_lexp_instant le1 absent ->
-          sem_lexp_instant le2 absent ->
-          sem_lexp_instant (Ebinop op le1 le2 ty) absent.
-
-    Definition sem_lexps_instant (les: list lexp) (vs: list value) :=
-      Forall2 sem_lexp_instant les vs.
-
-    Inductive sem_cexp_instant: cexp -> value -> Prop :=
-    | Smerge_true:
-        forall x t f c,
-          sem_var_instant x (present true_val) ->
-          sem_cexp_instant t (present c) ->
-          sem_cexp_instant f absent ->
-          sem_cexp_instant (Emerge x t f) (present c)
-    | Smerge_false:
-        forall x t f c,
-          sem_var_instant x (present false_val) ->
-          sem_cexp_instant t absent ->
-          sem_cexp_instant f (present c) ->
-          sem_cexp_instant (Emerge x t f) (present c)
-    | Smerge_abs:
-        forall x t f,
-          sem_var_instant x absent ->
-          sem_cexp_instant t absent ->
-          sem_cexp_instant f absent ->
-          sem_cexp_instant (Emerge x t f) absent
-    | Site_eq:
-        forall x t f c b ct cf,
-          sem_lexp_instant x (present c) ->
-          sem_cexp_instant t (present ct) ->
-          sem_cexp_instant f (present cf) ->
-          val_to_bool c = Some b ->
-          sem_cexp_instant (Eite x t f) (if b then present ct else present cf)
-    | Site_abs:
-        forall b t f,
-          sem_lexp_instant b absent ->
-          sem_cexp_instant t absent ->
-          sem_cexp_instant f absent ->
-          sem_cexp_instant (Eite b t f) absent
-    | Sexp:
-        forall e v,
-          sem_lexp_instant e v ->
-          sem_cexp_instant (Eexp e) v.
-
-  End InstantSemantics.
-
-  Lemma not_subrate_clock:
-    forall R ck,
-      ~ sem_clock_instant false R ck true.
-  Proof.
-    intros ** Sem; induction ck; inv Sem.
-    now apply IHck.
-  Qed.
-
-  Section InstantAnnotatedSemantics.
-
-    Variable base : bool.
-    Variable R: env.
-
-    Inductive sem_annotated_instant {A}
-              (sem_instant: bool -> env -> A -> value -> Prop)
-      : clock -> A -> value -> Prop :=
-    | Stick:
-        forall ck a c,
-          sem_instant base R a (present c) ->
-          sem_clock_instant base R ck true ->
-          sem_annotated_instant sem_instant ck a (present c)
-    | Sabs:
-        forall ck a,
-          sem_instant base R a absent ->
-          sem_clock_instant base R ck false ->
-          sem_annotated_instant sem_instant ck a absent.
-
-    Definition sem_laexp_instant := sem_annotated_instant sem_lexp_instant.
-    Definition sem_caexp_instant := sem_annotated_instant sem_cexp_instant.
-
-    Inductive sem_laexps_instant: clock -> list lexp -> list value -> Prop:=
-    | SLticks:
-        forall ck ces cs vs,
-          vs = map present cs ->
-          sem_lexps_instant base R ces vs ->
-          sem_clock_instant base R ck true ->
-          sem_laexps_instant ck ces vs
-    | SLabss:
-        forall ck ces vs,
-          vs = all_absent ces ->
-          sem_lexps_instant base R ces vs ->
-          sem_clock_instant base R ck false ->
-          sem_laexps_instant ck ces vs.
-    (* | SNil: *)
-    (*     forall ck, *)
-    (*       sem_laexps_instant ck [] []. *)
-
-  End InstantAnnotatedSemantics.
-
-  (** ** Liftings of instantaneous semantics *)
-
-  Section LiftSemantics.
-
-    Variable bk : stream bool.
-    Variable H : history.
-
-    Definition restr_hist (n: nat): env :=
-      PM.map (fun xs => xs n) H.
-    Hint Unfold restr_hist.
-
-    Definition lift {A B} (sem: bool -> env -> A -> B -> Prop)
-               x (ys: stream B): Prop :=
-      forall n, sem (bk n) (restr_hist n) x (ys n).
-    Hint Unfold lift.
-
-    Definition lift' {A B} (sem: env -> A -> B -> Prop) x (ys: stream B): Prop :=
-      forall n, sem (restr_hist n) x (ys n).
-    Hint Unfold lift'.
-
-    Definition sem_clock (ck: clock) (xs: stream bool): Prop :=
-      lift sem_clock_instant ck xs.
-
-    Definition sem_var (x: ident) (xs: stream value): Prop :=
-      lift' sem_var_instant x xs.
-
-    Definition sem_vars (x: idents) (xs: stream (list value)): Prop :=
-      lift' sem_vars_instant x xs.
-
-    Definition sem_laexp ck (e: lexp) (xs: stream value): Prop :=
-      lift (fun base R => sem_laexp_instant base R ck) e xs.
-
-    Definition sem_laexps (ck: clock) (e: list lexp) (xs: stream (list value)): Prop :=
-      lift (fun base R => sem_laexps_instant base R ck) e xs.
-
-    Definition sem_lexp (e: lexp) (xs: stream value): Prop :=
-      lift sem_lexp_instant e xs.
-
-    Definition sem_lexps (e: list lexp) (xs: stream (list value)): Prop :=
-      lift sem_lexps_instant e xs.
-
-    Definition sem_caexp ck (c: cexp) (xs: stream value): Prop :=
-      lift (fun base R => sem_caexp_instant base R ck) c xs.
-
-    Definition sem_cexp (c: cexp) (xs: stream value): Prop :=
-      lift sem_cexp_instant c xs.
-
-  End LiftSemantics.
-
-  (** ** Time-dependent semantics *)
-
-  Definition instant_same_clock (l : list value) : Prop :=
-    absent_list l \/ present_list l.
-
-  Definition same_clock (l_s : stream (list value)) : Prop :=
-    forall n, instant_same_clock (l_s n).
-
-  Definition clock_of (xss: stream (list value))(bs: stream bool): Prop :=
-    forall n,
-      present_list (xss n) <-> bs n = true.
-
-  Definition clock_of' (xss: stream (list value)) : stream bool :=
-    fun n => forallb (fun v => negb (v ==b absent)) (xss n).
-
-  Lemma clock_of_equiv:
-    forall xss, clock_of xss (clock_of' xss).
-  Proof.
-    split; intros H.
-    - unfold clock_of'.
-      rewrite forallb_forall.
-      intros; rewrite Bool.negb_true_iff.
-      rewrite not_equiv_decb_equiv.
-      eapply In_Forall in H; eauto.
-    - unfold clock_of' in H.
-      rewrite forallb_forall in H.
-      apply all_In_Forall; intros ** Hin E.
-      specialize (H _ Hin).
-      rewrite Bool.negb_true_iff, not_equiv_decb_equiv in H.
-      apply H; eauto.
-  Qed.
-
-  Lemma clock_of_equiv':
-    forall xss bk,
-      clock_of xss bk ->
-      bk ≈ clock_of' xss.
-  Proof.
-    intros ** H n; specialize (H n).
-    unfold clock_of'.
-    induction (xss n) as [|v]; simpl.
-    - apply H; constructor.
-    - destruct v.
-      + simpl.
-        rewrite <-Bool.not_true_iff_false, <-H.
-        inversion 1; auto.
-      + simpl.
-        apply IHl; rewrite <-H.
-        split; intro P.
-        * constructor; auto.
-          intro; discriminate.
-        * inv P; auto.
-  Qed.
-
-  (* Inductive next_reg: ident -> stream value -> memories -> Prop := *)
-  (*   post_mem_intro: *)
-  (*     forall x xs M mvs, *)
-  (*       mfind_mem x M = Some mvs -> *)
-  (*       mvs.(content) ≈ fby (sem_const mvs.(init)) xs -> *)
-  (*       next_reg x xs M . *)
-
   Inductive reset_regs: stream bool -> memories -> Prop :=
     reset_regs_intro:
       forall M rs,
@@ -343,15 +47,6 @@ Module Type SBSEMANTICS
             sub_inst x M M' ->
             reset_regs rs M') ->
         reset_regs rs M.
-
-  Definition reset_of_value (v: value) : bool :=
-    match v with
-    | present x => x ==b true_val
-    | absent => false
-    end.
-
-  Definition reset_of (xs: stream value) : stream bool :=
-    fun n => reset_of_value (xs n).
 
   Inductive mfby: ident -> val -> stream value -> memories -> stream value -> Prop :=
     mfby_intro:
@@ -483,59 +178,6 @@ Module Type SBSEMANTICS
 
   (** Morphisms properties *)
 
-  Add Parametric Morphism b A B sem H : (@lift b H A B sem)
-      with signature eq ==> @eq_str B ==> Basics.impl
-        as lift_eq_str.
-  Proof.
-    intros x xs xs' E Lift n.
-    rewrite <-E; auto.
-  Qed.
-
-  Add Parametric Morphism A B sem H : (@lift' H A B sem)
-      with signature eq ==> @eq_str B ==> Basics.impl
-        as lift'_eq_str.
-  Proof.
-    intros x xs xs' E Lift n.
-    rewrite <-E; auto.
-  Qed.
-
-  Add Parametric Morphism : clock_of
-      with signature eq_str ==> eq ==> Basics.impl
-        as clock_of_eq_str.
-  Proof.
-    unfold clock_of. intros ** E b Pres n.
-    split; intros H.
-    - apply Pres.
-      specialize (E n).
-      induction H; rewrite E; constructor; auto.
-    - apply Pres in H.
-      specialize (E n).
-      induction H; rewrite <-E; constructor; auto.
-  Qed.
-
-  (* Add Parametric Morphism : reset_of *)
-  (*     with signature eq_str ==> eq_str *)
-  (*       as reset_of_eq_str. *)
-  (* Proof. *)
-  (*   unfold reset_of. intros ** E n. *)
-  (*   now rewrite E. *)
-  (* Qed. *)
-
-  (* Add Parametric Morphism : reset_regs *)
-  (*     with signature eq_str ==> eq ==> Basics.impl *)
-  (*       as reset_regs_eq_str. *)
-  (* Proof. *)
-  (*   intros ** E M Rst. *)
-  (*   induction Rst; constructor; eauto. *)
-  (* Qed. *)
-
-  Add Parametric Morphism : same_clock
-      with signature eq_str ==> Basics.impl
-        as same_clock_eq_str.
-  Proof.
-    unfold same_clock; intros ** E ? ?; rewrite <-E; auto.
-  Qed.
-
   Add Parametric Morphism P b M: (sem_block P b M)
       with signature eq_str ==> eq_str ==> Basics.impl
         as sem_node_eq_str.
@@ -544,20 +186,6 @@ Module Type SBSEMANTICS
     inv Block.
     econstructor; eauto; intro; try rewrite <-E1; try rewrite <-E2; auto.
   Qed.
-
-  Ltac assert_const_length xss :=
-    match goal with
-      H: sem_vars _ _ xss |- _ =>
-      let H' := fresh in
-      let k := fresh in
-      let k' := fresh in
-      assert (wf_streams xss)
-        by (intros k k'; pose proof H as H';
-            unfold sem_vars, lift in *;
-            specialize (H k); specialize (H' k');
-            apply Forall2_length in H; apply Forall2_length in H';
-            now rewrite H in H')
-    end.
 
   Lemma sem_block_wf:
     forall P f M xss yss,
