NLustre/IsVariable.v
@@ -7,6 +7,7 @@ Open Scope list_scope.
 Require Import Velus.Common.
 Require Import Velus.Operators.
 Require Import Velus.Clocks.
+Require Import Velus.NLustre.NLExprSyntax.
 Require Import Velus.NLustre.NLSyntax.
 Require Import Velus.NLustre.IsDefined.
 Require Import Velus.NLustre.Memories.
@@ -24,12 +25,13 @@ Require Import Coq.Sorting.Permutation.
  *)
 
 Module Type ISVARIABLE
-       (Ids         : IDS)
-       (Op          : OPERATORS)
-       (Import Clks : CLOCKS    Ids)
-       (Import Syn  : NLSYNTAX  Ids Op Clks)
-       (Import Mem  : MEMORIES  Ids Op Clks Syn)
-       (Import IsD  : ISDEFINED Ids Op Clks Syn Mem).
+       (Ids            : IDS)
+       (Op             : OPERATORS)
+       (Import Clks    : CLOCKS    Ids)
+       (Import ExprSyn : NLEXPRSYNTAX  Op)
+       (Import Syn     : NLSYNTAX  Ids Op Clks ExprSyn)
+       (Import Mem     : MEMORIES  Ids Op Clks ExprSyn Syn)
+       (Import IsD     : ISDEFINED Ids Op Clks ExprSyn Syn Mem).
 
   Inductive Is_variable_in_eq : ident -> equation -> Prop :=
   | VarEqDef: forall x ck e,   Is_variable_in_eq x (EqDef x ck e)
@@ -350,12 +352,13 @@ Module Type ISVARIABLE
 End ISVARIABLE.
 
 Module IsVariableFun
-       (Ids  : IDS)
-       (Op   : OPERATORS)
-       (Clks : CLOCKS Ids)
-       (Syn  : NLSYNTAX  Ids Op Clks)
-       (Mem  : MEMORIES  Ids Op Clks Syn)
-       (IsD  : ISDEFINED Ids Op Clks Syn Mem)
-       <: ISVARIABLE Ids Op Clks Syn Mem IsD.
-  Include ISVARIABLE Ids Op Clks Syn Mem IsD.
+      (Ids     : IDS)
+       (Op      : OPERATORS)
+       (Clks    : CLOCKS    Ids)
+       (ExprSyn : NLEXPRSYNTAX  Op)
+       (Syn     : NLSYNTAX  Ids Op Clks ExprSyn)
+       (Mem     : MEMORIES  Ids Op Clks ExprSyn Syn)
+       (IsD     : ISDEFINED Ids Op Clks ExprSyn Syn Mem)
+       <: ISVARIABLE Ids Op Clks ExprSyn Syn Mem IsD.
+  Include ISVARIABLE Ids Op Clks ExprSyn Syn Mem IsD.
 End IsVariableFun.
