NLustre/NLExprSemantics.v
@@ -1,0 +1,776 @@
+Require Import List.
+Import List.ListNotations.
+Open Scope list_scope.
+
+Require Import Setoid.
+Require Import Morphisms.
+
+Require Import Velus.Common.
+Require Import Velus.Operators.
+Require Import Velus.Clocks.
+Require Import Velus.RMemory.
+Require Import Velus.NLustre.NLExprSyntax.
+Require Import Velus.NLustre.Stream.
+
+
+Module Type NLEXPRSEMANTICS
+       (Import Ids     : IDS)
+       (Import Op      : OPERATORS)
+       (Import OpAux   : OPERATORS_AUX    Op)
+       (Import Clks    : CLOCKS       Ids)
+       (Import ExprSyn : NLEXPRSYNTAX     Op)
+       (Import Str     : STREAM           Op OpAux).
+
+  (** ** Environment and history *)
+
+  (**
+
+An history maps variables to streams of values (the variables'
+histories). Taking a snapshot of the history at a given time yields an
+environment.
+
+   *)
+
+  Definition env := PM.t value.
+  Definition history := PM.t (stream value).
+
+  (** ** Instantaneous semantics *)
+
+  Section InstantSemantics.
+
+    Variable base: bool.
+    Variable R: env.
+
+    Inductive sem_var_instant: ident -> value -> Prop :=
+      Sv:
+        forall x v,
+          PM.find x R = Some v ->
+          sem_var_instant x v.
+
+    Definition sem_vars_instant (xs: list ident) (vs: list value) : Prop :=
+      Forall2 sem_var_instant xs vs.
+
+    Inductive sem_clock_instant: clock -> bool -> Prop :=
+    | Sbase:
+        sem_clock_instant Cbase base
+    | Son:
+        forall ck x c b,
+          sem_clock_instant ck true ->
+          sem_var_instant x (present c) ->
+          val_to_bool c = Some b ->
+          sem_clock_instant (Con ck x b) true
+    | Son_abs1:
+        forall ck x c,
+          sem_clock_instant ck false ->
+          sem_var_instant x absent ->
+          sem_clock_instant (Con ck x c) false
+    | Son_abs2:
+        forall ck x c b,
+          sem_clock_instant ck true ->
+          sem_var_instant x (present c) ->
+          val_to_bool c = Some b ->
+          sem_clock_instant (Con ck x (negb b)) false.
+
+    Inductive sem_lexp_instant: lexp -> value -> Prop:=
+    | Sconst:
+        forall c v,
+          v = (if base then present (sem_const c) else absent) ->
+          sem_lexp_instant (Econst c) v
+    | Svar:
+        forall x v ty,
+          sem_var_instant x v ->
+          sem_lexp_instant (Evar x ty) v
+    | Swhen_eq:
+        forall s x sc xc b,
+          sem_var_instant x (present xc) ->
+          sem_lexp_instant s (present sc) ->
+          val_to_bool xc = Some b ->
+          sem_lexp_instant (Ewhen s x b) (present sc)
+    | Swhen_abs1:
+        forall s x sc xc b,
+          sem_var_instant x (present xc) ->
+          val_to_bool xc = Some b ->
+          sem_lexp_instant s (present sc) ->
+          sem_lexp_instant (Ewhen s x (negb b)) absent
+    | Swhen_abs:
+        forall s x b,
+          sem_var_instant x absent ->
+          sem_lexp_instant s absent ->
+          sem_lexp_instant (Ewhen s x b) absent
+    | Sunop_eq:
+        forall le op c c' ty,
+          sem_lexp_instant le (present c) ->
+          sem_unop op c (typeof le) = Some c' ->
+          sem_lexp_instant (Eunop op le ty) (present c')
+    | Sunop_abs:
+        forall le op ty,
+          sem_lexp_instant le absent ->
+          sem_lexp_instant (Eunop op le ty) absent
+    | Sbinop_eq:
+        forall le1 le2 op c1 c2 c' ty,
+          sem_lexp_instant le1 (present c1) ->
+          sem_lexp_instant le2 (present c2) ->
+          sem_binop op c1 (typeof le1) c2 (typeof le2) = Some c' ->
+          sem_lexp_instant (Ebinop op le1 le2 ty) (present c')
+    | Sbinop_abs:
+        forall le1 le2 op ty,
+          sem_lexp_instant le1 absent ->
+          sem_lexp_instant le2 absent ->
+          sem_lexp_instant (Ebinop op le1 le2 ty) absent.
+
+    Definition sem_lexps_instant (les: list lexp) (vs: list value) :=
+      Forall2 sem_lexp_instant les vs.
+
+    Inductive sem_cexp_instant: cexp -> value -> Prop :=
+    | Smerge_true:
+        forall x t f c,
+          sem_var_instant x (present true_val) ->
+          sem_cexp_instant t (present c) ->
+          sem_cexp_instant f absent ->
+          sem_cexp_instant (Emerge x t f) (present c)
+    | Smerge_false:
+        forall x t f c,
+          sem_var_instant x (present false_val) ->
+          sem_cexp_instant t absent ->
+          sem_cexp_instant f (present c) ->
+          sem_cexp_instant (Emerge x t f) (present c)
+    | Smerge_abs:
+        forall x t f,
+          sem_var_instant x absent ->
+          sem_cexp_instant t absent ->
+          sem_cexp_instant f absent ->
+          sem_cexp_instant (Emerge x t f) absent
+    | Site_eq:
+        forall x t f c b ct cf,
+          sem_lexp_instant x (present c) ->
+          sem_cexp_instant t (present ct) ->
+          sem_cexp_instant f (present cf) ->
+          val_to_bool c = Some b ->
+          sem_cexp_instant (Eite x t f) (if b then present ct else present cf)
+    | Site_abs:
+        forall b t f,
+          sem_lexp_instant b absent ->
+          sem_cexp_instant t absent ->
+          sem_cexp_instant f absent ->
+          sem_cexp_instant (Eite b t f) absent
+    | Sexp:
+        forall e v,
+          sem_lexp_instant e v ->
+          sem_cexp_instant (Eexp e) v.
+
+  End InstantSemantics.
+
+  Section InstantAnnotatedSemantics.
+
+    Variable base : bool.
+    Variable R: env.
+
+    Inductive sem_annotated_instant {A}
+              (sem_instant: bool -> env -> A -> value -> Prop)
+      : clock -> A -> value -> Prop :=
+    | Stick:
+        forall ck a c,
+          sem_instant base R a (present c) ->
+          sem_clock_instant base R ck true ->
+          sem_annotated_instant sem_instant ck a (present c)
+    | Sabs:
+        forall ck a,
+          sem_instant base R a absent ->
+          sem_clock_instant base R ck false ->
+          sem_annotated_instant sem_instant ck a absent.
+
+    Definition sem_laexp_instant := sem_annotated_instant sem_lexp_instant.
+    Definition sem_caexp_instant := sem_annotated_instant sem_cexp_instant.
+
+    Inductive sem_laexps_instant: clock -> list lexp -> list value -> Prop:=
+    | SLticks:
+        forall ck ces cs vs,
+          vs = map present cs ->
+          sem_lexps_instant base R ces vs ->
+          sem_clock_instant base R ck true ->
+          sem_laexps_instant ck ces vs
+    | SLabss:
+        forall ck ces vs,
+          vs = all_absent ces ->
+          sem_lexps_instant base R ces vs ->
+          sem_clock_instant base R ck false ->
+          sem_laexps_instant ck ces vs.
+
+  End InstantAnnotatedSemantics.
+
+  (** ** Liftings of instantaneous semantics *)
+
+  Section LiftSemantics.
+
+    Variable bk : stream bool.
+    Variable H : history.
+
+    Definition restr_hist (n: nat): env :=
+      PM.map (fun xs => xs n) H.
+    Hint Unfold restr_hist.
+
+    Definition lift {A B} (sem: bool -> env -> A -> B -> Prop)
+               x (ys: stream B): Prop :=
+      forall n, sem (bk n) (restr_hist n) x (ys n).
+    Hint Unfold lift.
+
+    Definition lift' {A B} (sem: env -> A -> B -> Prop) x (ys: stream B): Prop :=
+      forall n, sem (restr_hist n) x (ys n).
+    Hint Unfold lift'.
+
+    Definition sem_clock (ck: clock) (xs: stream bool): Prop :=
+      lift sem_clock_instant ck xs.
+
+    Definition sem_var (x: ident) (xs: stream value): Prop :=
+      lift' sem_var_instant x xs.
+
+    Definition sem_vars (x: idents) (xs: stream (list value)): Prop :=
+      lift' sem_vars_instant x xs.
+
+    Definition sem_laexp ck (e: lexp) (xs: stream value): Prop :=
+      lift (fun base R => sem_laexp_instant base R ck) e xs.
+
+    Definition sem_laexps (ck: clock) (e: list lexp) (xs: stream (list value)): Prop :=
+      lift (fun base R => sem_laexps_instant base R ck) e xs.
+
+    Definition sem_lexp (e: lexp) (xs: stream value): Prop :=
+      lift sem_lexp_instant e xs.
+
+    Definition sem_lexps (e: list lexp) (xs: stream (list value)): Prop :=
+      lift sem_lexps_instant e xs.
+
+    Definition sem_caexp ck (c: cexp) (xs: stream value): Prop :=
+      lift (fun base R => sem_caexp_instant base R ck) c xs.
+
+    Definition sem_cexp (c: cexp) (xs: stream value): Prop :=
+      lift sem_cexp_instant c xs.
+
+  End LiftSemantics.
+
+  (** ** Time-dependent semantics *)
+
+  Definition instant_same_clock (l : list value) : Prop :=
+    absent_list l \/ present_list l.
+
+  Definition same_clock (l_s : stream (list value)) : Prop :=
+    forall n, instant_same_clock (l_s n).
+
+  Definition clock_of (xss: stream (list value))(bs: stream bool): Prop :=
+    forall n,
+      present_list (xss n) <-> bs n = true.
+
+  Definition clock_of' (xss: stream (list value)) : stream bool :=
+    fun n => forallb (fun v => negb (v ==b absent)) (xss n).
+
+  Lemma clock_of_equiv:
+    forall xss, clock_of xss (clock_of' xss).
+  Proof.
+    split; intros H.
+    - unfold clock_of'.
+      rewrite forallb_forall.
+      intros; rewrite Bool.negb_true_iff.
+      rewrite not_equiv_decb_equiv.
+      eapply In_Forall in H; eauto.
+    - unfold clock_of' in H.
+      rewrite forallb_forall in H.
+      apply all_In_Forall; intros ** Hin E.
+      specialize (H _ Hin).
+      rewrite Bool.negb_true_iff, not_equiv_decb_equiv in H.
+      apply H; eauto.
+  Qed.
+
+  Lemma clock_of_equiv':
+    forall xss bk,
+      clock_of xss bk ->
+      bk ≈ clock_of' xss.
+  Proof.
+    intros ** H n; specialize (H n).
+    unfold clock_of'.
+    induction (xss n) as [|v]; simpl.
+    - apply H; constructor.
+    - destruct v.
+      + simpl.
+        rewrite <-Bool.not_true_iff_false, <-H.
+        inversion 1; auto.
+      + simpl.
+        apply IHl; rewrite <-H.
+        split; intro P.
+        * constructor; auto.
+          intro; discriminate.
+        * inv P; auto.
+  Qed.
+
+  Definition reset_of_value (v: value) : bool :=
+    match v with
+    | present x => x ==b true_val
+    | absent => false
+    end.
+
+  Definition reset_of (xs: stream value) : stream bool :=
+    fun n => reset_of_value (xs n).
+
+  (** Morphisms properties *)
+
+  Add Parametric Morphism b A B sem H : (@lift b H A B sem)
+      with signature eq ==> @eq_str B ==> Basics.impl
+        as lift_eq_str.
+  Proof.
+    intros x xs xs' E Lift n.
+    rewrite <-E; auto.
+  Qed.
+
+  Add Parametric Morphism A B sem H : (@lift' H A B sem)
+      with signature eq ==> @eq_str B ==> Basics.impl
+        as lift'_eq_str.
+  Proof.
+    intros x xs xs' E Lift n.
+    rewrite <-E; auto.
+  Qed.
+
+  Add Parametric Morphism : clock_of
+      with signature eq_str ==> eq ==> Basics.impl
+        as clock_of_eq_str.
+  Proof.
+    unfold clock_of. intros ** E b Pres n.
+    split; intros H.
+    - apply Pres.
+      specialize (E n).
+      induction H; rewrite E; constructor; auto.
+    - apply Pres in H.
+      specialize (E n).
+      induction H; rewrite <-E; constructor; auto.
+  Qed.
+
+  (* Add Parametric Morphism : reset_of *)
+  (*     with signature eq_str ==> eq_str *)
+  (*       as reset_of_eq_str. *)
+  (* Proof. *)
+  (*   unfold reset_of. intros ** E n. *)
+  (*   now rewrite E. *)
+  (* Qed. *)
+
+  (* Add Parametric Morphism : reset_regs *)
+  (*     with signature eq_str ==> eq ==> Basics.impl *)
+  (*       as reset_regs_eq_str. *)
+  (* Proof. *)
+  (*   intros ** E M Rst. *)
+  (*   induction Rst; constructor; eauto. *)
+  (* Qed. *)
+
+  Add Parametric Morphism : same_clock
+      with signature eq_str ==> Basics.impl
+        as same_clock_eq_str.
+  Proof.
+    unfold same_clock; intros ** E ? ?; rewrite <-E; auto.
+  Qed.
+
+  (** ** Clocking property *)
+
+  Lemma not_subrate_clock:
+    forall R ck,
+      ~ sem_clock_instant false R ck true.
+  Proof.
+    intros ** Sem; induction ck; inv Sem.
+    now apply IHck.
+  Qed.
+
+  Lemma present_not_absent_list:
+    forall xs (vs: list val),
+      instant_same_clock xs ->
+      ~ absent_list xs ->
+      present_list xs.
+  Proof.
+    intros ** Hsamexs Hnabs.
+    now destruct Hsamexs.
+  Qed.
+
+  Lemma sem_vars_gt0:
+    forall H (xs: list (ident * type)) ls,
+      0 < length xs ->
+      sem_vars H (map fst xs) ls ->
+      forall n, 0 < length (ls n).
+  Proof.
+    intros ** Hgt0 Hsem n.
+    specialize (Hsem n).
+    apply Forall2_length in Hsem.
+    rewrite map_length in Hsem.
+    now rewrite Hsem in Hgt0.
+  Qed.
+
+  Ltac assert_const_length xss :=
+    match goal with
+      H: sem_vars _ _ xss |- _ =>
+      let H' := fresh in
+      let k := fresh in
+      let k' := fresh in
+      assert (wf_streams xss)
+        by (intros k k'; pose proof H as H';
+            unfold sem_vars, lift in *;
+            specialize (H k); specialize (H' k');
+            apply Forall2_length in H; apply Forall2_length in H';
+            now rewrite H in H')
+    end.
+
+  (** ** Determinism of the semantics *)
+
+  (** *** Instantaneous semantics *)
+
+  Section InstantDeterminism.
+
+    Variable base: bool.
+    Variable R: env.
+
+    Lemma sem_var_instant_det:
+      forall x v1 v2,
+        sem_var_instant R x v1
+        -> sem_var_instant R x v2
+        -> v1 = v2.
+    Proof.
+      intros x v1 v2 H1 H2.
+      inversion_clear H1 as [Hf1];
+        inversion_clear H2 as [Hf2];
+        congruence.
+    Qed.
+
+    Lemma sem_clock_instant_det:
+      forall ck v1 v2,
+        sem_clock_instant base R ck v1
+        -> sem_clock_instant base R ck v2
+        -> v1 = v2.
+    Proof.
+      induction ck; repeat inversion 1; subst; intuition;
+        try repeat progress match goal with
+                            | H1: sem_clock_instant ?bk ?R ?ck ?l,
+                                  H2: sem_clock_instant ?bk ?R ?ck ?r |- _ =>
+                              apply IHck with (1:=H1) in H2; discriminate
+                            | H1: sem_var_instant ?R ?i (present ?l),
+                                  H2: sem_var_instant ?R ?i (present ?r) |- _ =>
+                              apply sem_var_instant_det with (1:=H1) in H2;
+                                injection H2; intro; subst
+                            | H1: val_to_bool _ = Some ?b, H2: val_to_bool _ = _ |- _ =>
+                              rewrite H1 in H2; destruct b; discriminate
+                            end.
+    Qed.
+
+    Lemma sem_lexp_instant_det:
+      forall e v1 v2,
+        sem_lexp_instant base R e v1
+        -> sem_lexp_instant base R e v2
+        -> v1 = v2.
+    Proof.
+      induction e (* using lexp_ind2 *);
+        try now (do 2 inversion_clear 1);
+        match goal with
+        | H1:sem_var_instant ?R ?e (present ?b1),
+             H2:sem_var_instant ?R ?e (present ?b2),
+                H3: ?b1 <> ?b2 |- _ =>
+          exfalso; apply H3;
+            cut (present (Vbool b1) = present (Vbool b2)); [now injection 1|];
+              eapply sem_var_instant_det; eassumption
+        | H1:sem_var_instant ?R ?e ?v1,
+             H2:sem_var_instant ?R ?e ?v2 |- ?v1 = ?v2 =>
+          eapply sem_var_instant_det; eassumption
+        | H1:sem_var_instant ?R ?e (present _),
+             H2:sem_var_instant ?R ?e absent |- _ =>
+          apply (sem_var_instant_det _ _ _ _ H1) in H2;
+            discriminate
+        | _ => auto
+        end.
+      - (* Econst *)
+        do 2 inversion_clear 1; destruct base; congruence.
+      - (* Ewhen *)
+        intros v1 v2 Hsem1 Hsem2.
+        inversion Hsem1; inversion Hsem2; subst;
+          repeat progress match goal with
+                          | H1:sem_lexp_instant ?b ?R ?e ?v1,
+                               H2:sem_lexp_instant ?b ?R ?e ?v2 |- _ =>
+                            apply IHe with (1:=H1) in H2
+                          | H1:sem_var_instant ?R ?i ?v1,
+                               H2:sem_var_instant ?R ?i ?v2 |- _ =>
+                            apply sem_var_instant_det with (1:=H1) in H2
+                          | H1:sem_unop _ _ _ = Some ?v1,
+                               H2:sem_unop _ _ _ = Some ?v2 |- _ =>
+                            rewrite H1 in H2; injection H2; intro; subst
+                          | Hp:present _ = present _ |- _ =>
+                            injection Hp; intro; subst
+                          | H1:val_to_bool _ = Some _,
+                               H2:val_to_bool _ = Some (negb _) |- _ =>
+                            rewrite H2 in H1; exfalso; injection H1;
+                              now apply Bool.no_fixpoint_negb
+                          end; subst; try easy.
+      - (* Eunop *)
+        intros v1 v2 Hsem1 Hsem2.
+        inversion_clear Hsem1; inversion_clear Hsem2;
+          repeat progress match goal with
+                          | H1:sem_lexp_instant _ _ e _, H2:sem_lexp_instant _ _ e _ |- _ =>
+                            apply IHe with (1:=H1) in H2; inversion H2; subst
+                          | H1:sem_unop _ _ _ = _, H2:sem_unop _ _ _ = _ |- _ =>
+                            rewrite H1 in H2; injection H2; intro; subst
+                          | H1:sem_lexp_instant _ _ _ (present _),
+                               H2:sem_lexp_instant _ _ _ absent |- _ =>
+                            apply IHe with (1:=H1) in H2
+                          end; try easy.
+      - (* Ebinop *)
+        intros v1 v2 Hsem1 Hsem2.
+        inversion_clear Hsem1; inversion_clear Hsem2;
+          repeat progress match goal with
+                          | H1:sem_lexp_instant _ _ e1 _, H2:sem_lexp_instant _ _ e1 _ |- _ =>
+                            apply IHe1 with (1:=H1) in H2
+                          | H1:sem_lexp_instant _ _ e2 _, H2:sem_lexp_instant _ _ e2 _ |- _ =>
+                            apply IHe2 with (1:=H1) in H2
+                          | H1:sem_binop _ _ _ _ _ = Some ?v1,
+                               H2:sem_binop _ _ _ _ _ = Some ?v2 |- _ =>
+                            rewrite H1 in H2; injection H2; intro; subst
+                          | H:present _ = present _ |- _ => injection H; intro; subst
+                          end; subst; try easy.
+    Qed.
+
+    Lemma sem_laexp_instant_det:
+      forall ck e v1 v2,
+        sem_laexp_instant base R ck e v1
+        -> sem_laexp_instant base R ck e v2
+        -> v1 = v2.
+    Proof.
+      intros ck e v1 v2.
+      do 2 inversion_clear 1;
+        match goal with
+        | H1:sem_lexp_instant _ _ _ _, H2:sem_lexp_instant _ _ _ _ |- _ =>
+          eapply sem_lexp_instant_det; eassumption
+        | H1:sem_clock_instant _ _ _ ?T, H2:sem_clock_instant _ _ _ ?F |- _ =>
+          assert (T = F) by (eapply sem_clock_instant_det; eassumption);
+            try discriminate
+        end; auto.
+    Qed.
+
+    Lemma sem_lexps_instant_det:
+      forall les cs1 cs2,
+        sem_lexps_instant base R les cs1 ->
+        sem_lexps_instant base R les cs2 ->
+        cs1 = cs2.
+    Proof.
+      intros les cs1 cs2. apply Forall2_det. apply sem_lexp_instant_det.
+    Qed.
+
+    Lemma sem_laexps_instant_det:
+      forall ck e v1 v2,
+        sem_laexps_instant base R ck e v1
+        -> sem_laexps_instant base R ck e v2
+        -> v1 = v2.
+    Proof.
+      intros until v2.
+      do 2 inversion_clear 1;
+        match goal with
+        | H1: sem_lexps_instant _ _ _ _, H2: sem_lexps_instant _ _ _ _ |- _ =>
+          eapply sem_lexps_instant_det; eauto
+        | H1:sem_clock_instant _ _ _ ?T, H2:sem_clock_instant _ _ _ ?F |- _ =>
+          let H := fresh in
+          assert (H: T = F) by (eapply sem_clock_instant_det; eassumption);
+            try discriminate H
+        end; congruence.
+    Qed.
+
+    Lemma sem_cexp_instant_det:
+      forall e v1 v2,
+        sem_cexp_instant base R e v1
+        -> sem_cexp_instant base R e v2
+        -> v1 = v2.
+    Proof.
+      induction e;
+        do 2 inversion_clear 1;
+        try repeat progress match goal with
+                            | H1: sem_cexp_instant ?bk ?R ?e ?l,
+                                  H2: sem_cexp_instant ?bk ?R ?e ?r |- _ =>
+                              apply IHe1 with (1:=H1) in H2
+                                                         || apply IHe2 with (1:=H1) in H2;
+                                injection H2; intro; subst
+                            | H1: sem_var_instant ?R ?i (present true_val),
+                                  H2: sem_var_instant ?R ?i (present false_val) |- _ =>
+                              apply sem_var_instant_det with (1:=H1) in H2;
+                                exfalso; injection H2; now apply true_not_false_val
+                            | H1: sem_lexp_instant ?bk ?R ?l ?v1,
+                                  H2: sem_lexp_instant ?bk ?R ?l ?v2 |- _ =>
+                              apply sem_lexp_instant_det with (1:=H1) in H2;
+                                discriminate || injection H2; intro; subst
+                            | H1: sem_var_instant ?R ?i (present _),
+                                  H2: sem_var_instant ?R ?i absent |- _ =>
+                              apply sem_var_instant_det with (1:=H1) in H2; discriminate
+                            | H1: val_to_bool _ = Some _,
+                                  H2:val_to_bool _ = Some _ |- _ =>
+                              rewrite H1 in H2; injection H2; intro; subst
+                            end; auto.
+      eapply sem_lexp_instant_det; eassumption.
+    Qed.
+
+    Lemma sem_caexp_instant_det:
+      forall ck e v1 v2,
+        sem_caexp_instant base R ck e v1
+        -> sem_caexp_instant base R ck e v2
+        -> v1 = v2.
+    Proof.
+      intros until v2.
+      do 2 inversion_clear 1;
+        match goal with
+        | H1: sem_cexp_instant _ _ _ _,
+              H2: sem_cexp_instant _ _ _ _ |- _ =>
+          eapply sem_cexp_instant_det; eassumption
+        | H1:sem_clock_instant _ _ _ ?T,
+             H2:sem_clock_instant _ _ _ ?F |- _ =>
+          let H := fresh in
+          assert (H: T = F) by (eapply sem_clock_instant_det; eassumption);
+            try discriminate H
+        end; congruence.
+    Qed.
+
+  End InstantDeterminism.
+
+  (** *** Lifted semantics *)
+
+  Section LiftDeterminism.
+
+    Variable bk : stream bool.
+    Variable H : history.
+
+    Require Import Logic.FunctionalExtensionality.
+
+    Lemma lift_det:
+      forall {A B} (P: bool -> env -> A -> B -> Prop) (bk: stream bool)
+        x (xs1 xs2 : stream B),
+        (forall b R v1 v2, P b R x v1 -> P b R x v2 -> v1 = v2) ->
+        lift bk H P x xs1 -> lift bk H P x xs2 -> xs1 = xs2.
+    Proof.
+      intros ** Hpoint H1 H2.
+      extensionality n. specialize (H1 n). specialize (H2 n).
+      eapply Hpoint; eassumption.
+    Qed.
+
+    Lemma lift'_det:
+      forall {A B} (P: env -> A -> B -> Prop)
+        x (xs1 xs2 : stream B),
+        (forall R v1 v2, P R x v1 -> P R x v2 -> v1 = v2) ->
+        lift' H P x xs1 -> lift' H P x xs2 -> xs1 = xs2.
+    Proof.
+      intros ** Hpoint H1 H2.
+      extensionality n. specialize (H1 n). specialize (H2 n).
+      eapply Hpoint; eassumption.
+    Qed.
+
+    Ltac apply_lift sem_det :=
+      intros; eapply lift_det; try eassumption;
+      compute; intros; eapply sem_det; eauto.
+
+    Ltac apply_lift' sem_det :=
+      intros; eapply lift'_det; try eassumption;
+      compute; intros; eapply sem_det; eauto.
+
+    Lemma sem_var_det:
+      forall x xs1 xs2,
+        sem_var H x xs1 -> sem_var H x xs2 -> xs1 = xs2.
+    Proof.
+      apply_lift' sem_var_instant_det.
+    Qed.
+
+    Lemma sem_clock_det:
+      forall ck bs1 bs2,
+        sem_clock bk H ck bs1 -> sem_clock bk H ck bs2 -> bs1 = bs2.
+    Proof.
+      apply_lift sem_clock_instant_det.
+    Qed.
+
+    Lemma sem_lexp_det:
+      forall e xs1 xs2,
+        sem_lexp bk H e xs1 -> sem_lexp bk H e xs2 -> xs1 = xs2.
+    Proof.
+      apply_lift sem_lexp_instant_det.
+    Qed.
+
+    Lemma sem_lexps_det:
+      forall les cs1 cs2,
+        sem_lexps bk H les cs1 ->
+        sem_lexps bk H les cs2 ->
+        cs1 = cs2.
+    Proof.
+      apply_lift sem_lexps_instant_det.
+    Qed.
+
+    Lemma sem_laexp_det:
+      forall ck e xs1 xs2,
+        sem_laexp bk H ck e xs1 -> sem_laexp bk H ck e xs2 -> xs1 = xs2.
+    Proof.
+      apply_lift sem_laexp_instant_det.
+    Qed.
+
+    Lemma sem_laexps_det:
+      forall ck e xs1 xs2,
+        sem_laexps bk H ck e xs1 -> sem_laexps bk H ck e xs2 -> xs1 = xs2.
+    Proof.
+      apply_lift sem_laexps_instant_det.
+    Qed.
+
+    Lemma sem_cexp_det:
+      forall c xs1 xs2,
+        sem_cexp bk H c xs1 -> sem_cexp bk H c xs2 -> xs1 = xs2.
+    Proof.
+      apply_lift sem_cexp_instant_det.
+    Qed.
+
+    Lemma sem_caexp_det:
+      forall ck c xs1 xs2,
+        sem_caexp bk H ck c xs1 -> sem_caexp bk H ck c xs2 -> xs1 = xs2.
+    Proof.
+      apply_lift sem_caexp_instant_det.
+    Qed.
+
+  (* XXX: every semantics definition, including [sem_var] which doesn't
+need it, takes a base clock value or base clock stream, except
+[sem_var_instant]. For uniformity, we may want to pass a (useless)
+clock to [sem_var_instant] too. *)
+
+  End LiftDeterminism.
+
+  Ltac sem_det :=
+    match goal with
+    | H1: sem_clock_instant ?bk ?H ?C ?X,
+          H2: sem_clock_instant ?bk ?H ?C ?Y |- ?X = ?Y =>
+      eapply sem_clock_instant_det; eexact H1 || eexact H2
+    | H1: sem_clock ?bk ?H ?C ?X,
+          H2: sem_clock ?bk ?H ?C ?Y |- ?X = ?Y =>
+      eapply sem_clock_det; eexact H1 || eexact H2
+    | H1: sem_cexp_instant ?bk ?H ?C ?X,
+          H2: sem_cexp_instant ?bk ?H ?C ?Y |- ?X = ?Y =>
+      eapply sem_cexp_instant_det; eexact H1 || eexact H2
+    | H1: sem_cexp ?bk ?H ?C ?X,
+          H2: sem_cexp ?bk ?H ?C ?Y |- ?X = ?Y =>
+      eapply sem_cexp_det; eexact H1 || eexact H2
+    | H1: sem_lexps_instant ?bk ?H ?C ?X,
+          H2: sem_lexps_instant ?bk ?H ?C ?Y |- ?X = ?Y =>
+      eapply sem_lexps_instant_det; eexact H1 || eexact H2
+    | H1: sem_lexps ?bk ?H ?C ?X,
+          H2: sem_lexps ?bk ?H ?C ?Y |- ?X = ?Y =>
+      eapply sem_lexps_det; eexact H1 || eexact H2
+    | H1: sem_laexps_instant ?bk ?H ?ck ?C ?X,
+          H2: sem_laexps_instant ?bk ?H ?ck ?C ?Y |- ?X = ?Y =>
+      eapply sem_laexps_instant_det; eexact H1 || eexact H2
+    | H1: sem_laexps ?bk ?H ?ck ?C ?X,
+          H2: sem_laexps ?bk ?H ?ck ?C ?Y |- ?X = ?Y =>
+      eapply sem_laexps_det; eexact H1 || eexact H2
+    | H1: sem_lexp_instant ?bk ?H ?C ?X,
+          H2: sem_lexp_instant ?bk ?H ?C ?Y |- ?X = ?Y =>
+      eapply sem_lexp_instant_det; eexact H1 || eexact H2
+    | H1: sem_lexp ?bk ?H ?C ?X,
+          H2: sem_lexp ?bk ?H ?C ?Y |- ?X = ?Y =>
+      eapply sem_lexp_det; eexact H1 || eexact H2
+    | H1: sem_laexp_instant ?bk ?H ?CK ?C ?X,
+          H2: sem_laexp_instant ?bk ?H ?CK ?C ?Y |- ?X = ?Y =>
+      eapply sem_laexp_instant_det; eexact H1 || eexact H2
+    | H1: sem_laexp ?bk ?H ?CK ?C ?X,
+          H2: sem_laexp ?bk ?H ?CK ?C ?Y |- ?X = ?Y =>
+      eapply sem_laexp_det; eexact H1 || eexact H2
+    | H1: sem_var_instant ?C ?X,
+          H2: sem_var_instant ?C ?Y |- ?X = ?Y =>
+      eapply sem_var_instant_det; eexact H1 || eexact H2
+    | H1: sem_var ?H ?C ?X,
+          H2: sem_var ?H ?C ?Y |- ?X = ?Y =>
+      eapply sem_var_det; eexact H1 || eexact H2
+    end.
+
+End NLEXPRSEMANTICS.
