NLustre/NLExprSyntax.v
@@ -1,0 +1,35 @@
+Require Import Velus.Common.
+Require Import Velus.Operators.
+
+(** * The NLustre dataflow language *)
+
+Module Type NLEXPRSYNTAX (Import Op: OPERATORS).
+
+  (** ** Expressions *)
+
+  Inductive lexp : Type :=
+  | Econst : const -> lexp
+  | Evar   : ident -> type -> lexp
+  | Ewhen  : lexp -> ident -> bool -> lexp
+  | Eunop  : unop -> lexp -> type -> lexp
+  | Ebinop : binop -> lexp -> lexp -> type -> lexp.
+
+  Definition lexps := list lexp.
+
+  (** ** Control expressions *)
+
+  Inductive cexp : Type :=
+  | Emerge : ident -> cexp -> cexp -> cexp
+  | Eite   : lexp -> cexp -> cexp -> cexp
+  | Eexp   : lexp -> cexp.
+
+  Fixpoint typeof (le: lexp): type :=
+    match le with
+    | Econst c => type_const c
+    | Evar _ ty
+    | Eunop _ _ ty
+    | Ebinop _ _ _ ty => ty
+    | Ewhen e _ _ => typeof e
+    end.
+
+End NLEXPRSYNTAX.
