NLustre/NoDup.v
@@ -7,6 +7,7 @@ Require Import Velus.Common.
 Require Import Velus.Operators.
 Require Import Velus.Clocks.
 Require Import Velus.NLustre.NLSyntax.
+Require Import Velus.NLustre.NLExprSyntax.
 Require Import Velus.NLustre.IsVariable.
 Require Import Velus.NLustre.IsDefined.
 Require Import Velus.NLustre.Memories.
@@ -31,13 +32,14 @@ this generically amounts to:
  *)
 
 Module Type NODUP
-       (Ids         : IDS)
-       (Op          : OPERATORS)
-       (Import Clks : CLOCKS     Ids)
-       (Import Syn  : NLSYNTAX   Ids Op Clks)
-       (Import Mem  : MEMORIES   Ids Op Clks Syn)
-       (Import IsD  : ISDEFINED  Ids Op Clks Syn Mem)
-       (Import IsV  : ISVARIABLE Ids Op Clks Syn Mem IsD).
+       (Ids            : IDS)
+       (Op             : OPERATORS)
+       (Import Clks    : CLOCKS     Ids)
+       (Import ExprSyn : NLEXPRSYNTAX   Op)
+       (Import Syn     : NLSYNTAX   Ids Op Clks ExprSyn)
+       (Import Mem     : MEMORIES   Ids Op Clks ExprSyn Syn)
+       (Import IsD     : ISDEFINED  Ids Op Clks ExprSyn Syn Mem)
+       (Import IsV     : ISVARIABLE Ids Op Clks ExprSyn Syn Mem IsD).
 
   Inductive NoDup_defs : list equation -> Prop :=
   | NDDNil: NoDup_defs nil
@@ -160,15 +162,16 @@ Module Type NODUP
 End NODUP.
 
 Module NoDupFun
-       (Ids  : IDS)
-       (Op   : OPERATORS)
-       (Clks : CLOCKS Ids)
-       (Syn  : NLSYNTAX   Ids Op Clks)
-       (Mem  : MEMORIES   Ids Op Clks Syn)
-       (IsD  : ISDEFINED  Ids Op Clks Syn Mem)
-       (IsV  : ISVARIABLE Ids Op Clks Syn Mem IsD)
-       <: NODUP Ids Op Clks Syn Mem IsD IsV.
+       (Ids     : IDS)
+       (Op      : OPERATORS)
+       (Clks    : CLOCKS Ids)
+       (ExprSyn : NLEXPRSYNTAX   Op)
+       (Syn     : NLSYNTAX   Ids Op Clks ExprSyn)
+       (Mem     : MEMORIES   Ids Op Clks ExprSyn Syn)
+       (IsD     : ISDEFINED  Ids Op Clks ExprSyn Syn Mem)
+       (IsV     : ISVARIABLE Ids Op Clks ExprSyn Syn Mem IsD)
+       <: NODUP Ids Op Clks ExprSyn Syn Mem IsD IsV.
 
-  Include NODUP Ids Op Clks Syn Mem IsD IsV.
+  Include NODUP Ids Op Clks ExprSyn Syn Mem IsD IsV.
 
 End NoDupFun.
